SEARNarith.sml
@@ -1,0 +1,221 @@
+local
+val lemma = 
+ fVar_Inst 
+[("P",([("A",mem_sort$ Pow $ Cross N (mk_set "X"))],
+“IN(Pair(O,a:mem(X)),A) &
+ (!n x.IN(Pair(n,x),A) ==> IN(Pair(Eval(SUC,n),Eval(f,x)),A))”))] 
+(IN_def_P_expand |> qspecl [‘Pow(N * X)’]) 
+val As_def = lemma |> ex2fsym0 "As" ["a","f"] |> conjE1 
+                   |> gen_all |> GSYM
+val U_ex_lemma = fVar_Inst 
+[("P",([("nx",mem_sort $ Cross N (mk_set "X"))],
+“IN(nx,Eval(BI(N * X),As(a0,f)))”))]
+(Thm_2_4 |> qspecl [‘N * X’]) 
+|> conv_rule $ once_depth_fconv no_conv 
+$ rewr_fconv (spec_all BI_property)
+|> conv_rule $ once_depth_fconv no_conv 
+$ rewr_fconv (spec_all As_def) |> gen_all
+val rel_ex_lemma = 
+fVar_Inst 
+[("P",([("n",mem_sort N),("x",mem_sort (mk_set "X"))],
+“?r.Eval(u0:U-> N * X,r) = Pair(n,x)”))]
+(AX1 |> qspecl [‘N’,‘X’]) |> uex_expand
+val imp_ind_l = 
+fVar_Inst 
+[("P",([("n",mem_sort N)],
+“!x.Holds(R:N->X,n,x) ==> Holds(R,Eval(SUC,n),Eval(f,x))”))]
+N_ind_P
+val O_case_u_l = 
+fVar_Inst 
+[("P",([("nx",mem_sort $ Cross N (mk_set "X"))],
+“Holds(R,Eval(pi1(N,X),nx),Eval(pi2(N,X),nx)) & 
+ ~(Eval(pi1(N,X),nx) = O & Eval(pi2(N,X),nx) = x)”))] 
+(IN_def_P_expand |> qspecl [‘(N * X)’]) 
+val ex_R_ss = 
+fVar_Inst 
+[("P",([("mr",mem_sort $ Cross N (mk_set "X"))],
+“Holds(R,Eval(pi1(N,X),mr),Eval(pi2(N,X),mr)) &
+ !n. Eval(pi1(N,X),mr) = Eval(SUC,n) ==>
+ ?r0.Holds(R,n,r0) & Eval(pi2(N,X),mr) = Eval(f:X->X,r0)”))] 
+(IN_def_P_expand |> qspecl [‘(N * X)’]) 
+val u_R_ss1 = 
+fVar_Inst 
+[("P",([("mr",mem_sort $ Cross N (mk_set "X"))],
+“Holds(R,Eval(pi1(N,X),mr),Eval(pi2(N,X),mr)) &
+ (!x'.Holds(R,Eval(pi1(N,X),mr),x') ==> x' = Eval(pi2(N,X),mr))”))] 
+(IN_def_P_expand |> qspecl [‘(N * X)’]) 
+val ex_ind_l = 
+fVar_Inst 
+[("P",([("n",mem_sort N)],
+“?x.Holds(R:N->X,n,x)”))]
+N_ind_P
+in
+val Nind_ex = prove_store("Nind_ex",
+e0
+(rpt strip_tac >> 
+ qspecl_then [‘X’,‘a’,‘f’] (x_choosel_then ["U","u0"] 
+ strip_assume_tac) U_ex_lemma >>
+ strip_assume_tac rel_ex_lemma >> pop_assum (K all_tac) >>
+ (*qexists_tac ‘R’ >> *)
+ qby_tac 
+ ‘!n x. Holds(R,n,x) <=>
+  !ss. IN(Pair(O,a),ss) &
+       (!n x. IN(Pair(n,x),ss) ==>
+              IN(Pair(Eval(SUC,n),Eval(f,x)),ss)) ==>
+        IN(Pair(n,x),ss)’
+ >-- (arw[] >> rpt strip_tac >>
+ fconv_tac 
+ (rand_fconv no_conv 
+ $ basic_once_fconv no_conv (rewr_fconv (eq_sym "mem"))) >> rw[]) >>
+ pop_assum mp_tac >> pop_assum (K all_tac) >> 
+ pop_assum (K all_tac) >> strip_tac >>
+ qby_tac 
+ ‘Holds(R,O,a)’ >-- (arw[] >> rpt strip_tac) >>
+ qby_tac
+ ‘!n x. Holds(R,n,x) ==> Holds(R,Eval(SUC,n),Eval(f,x))’
+ >-- (match_mp_tac imp_ind_l (* irule bug *)>> strip_tac (* 2 *)
+     (*0 case*)
+     >-- (rpt strip_tac >>
+         qsuff_tac ‘Holds(R, O, x') ==>
+         Holds(R, Eval(SUC, O), Eval(f, x'))’ 
+         >-- (rpt strip_tac >> first_assum drule >> arw[]) >>
+         arw[] >> rpt strip_tac >> first_assum irule >>
+         last_assum $ irule o iffLR >> arw[]) >>
+     rpt strip_tac >> arw[] >> 
+     rpt strip_tac >> first_assum irule >>
+     qpick_x_assum ‘Holds(R, Eval(SUC, n'), x')’ mp_tac >> 
+     arw[] >> rpt strip_tac >> first_assum irule >> arw[]) >>
+ qby_tac ‘!x. Holds(R,O,x) ==> x = a’
+ >-- (rpt strip_tac >> ccontra_tac >>
+      qsuff_tac ‘?ss. IN(Pair(O,a),ss) & 
+      (!n x.IN(Pair(n,x),ss) ==> IN(Pair(Eval(SUC,n),Eval(f,x)),ss)) &
+      ~(IN(Pair(O,x),ss))’
+      >-- (last_assum (drule o iffLR) >> rpt strip_tac >>
+          qsuff_tac ‘IN(Pair(O, x), ss)’
+          >-- arw[] >>
+          first_x_assum irule >> arw[]) >>
+      x_choose_then "ss" strip_assume_tac O_case_u_l >>
+      pop_assum (K all_tac) >>
+      qby_tac ‘~(IN(Pair(O,x),ss))’
+      >-- (pop_assum (assume_tac o GSYM) >> once_arw[] >>
+          rw[Pair_def]) >>
+      qby_tac ‘IN(Pair(O,a),ss)’
+      >-- (pop_assum (K all_tac) >> pop_assum (assume_tac o GSYM) >>
+           once_arw[] >> rw[Pair_def] >> arw[] >>
+           flip_tac >> first_x_assum accept_tac) >>
+      qexists_tac ‘ss’ >> arw[] >>
+      pop_assum (K all_tac) >> pop_assum (K all_tac) >>
+      pop_assum (assume_tac o GSYM) >> strip_tac >> strip_tac >> 
+      once_arw[] >> rw[Pair_def] >> rpt strip_tac >-- 
+      (first_x_assum irule >> arw[]) >>
+      rw[SUC_NONZERO]) >>
+ qby_tac ‘!ss.IN(Pair(O,a),ss) &
+      (!n x.IN(Pair(n,x),ss) ==> IN(Pair(Eval(SUC,n),Eval(f,x)),ss)) ==>
+      !n x. Holds(R,n,x) ==> IN(Pair(n,x),ss)’
+ >-- (once_arw[] >> rpt strip_tac >> first_x_assum irule >>
+     arw[]) >>
+ x_choose_then "ss" strip_assume_tac ex_R_ss >>
+ pop_assum (K all_tac) >>
+ pop_assum (assume_tac o GSYM) >>
+ qby_tac ‘!n x. Holds(R,n,x) ==> IN(Pair(n,x),ss)’
+ >-- (first_x_assum match_mp_tac >> once_arw[] >>
+      rw[Pair_def] >> strip_tac (* 2 *)
+      >-- (strip_tac >-- first_x_assum accept_tac >>
+           flip_tac >> rw[SUC_NONZERO]) >>
+      rpt strip_tac (*2  *)
+      >-- (first_x_assum irule >> first_x_assum accept_tac) >>
+      qexists_tac ‘x'’ >> rw[] >>
+      fs[SUC_eq_eq]) >>
+ pop_assum mp_tac >>
+ last_x_assum mp_tac >> last_x_assum mp_tac >> 
+ last_x_assum (assume_tac o GSYM) >> once_arw[] >>
+ rw[Pair_def] >> rpt strip_tac >>
+ qby_tac
+ ‘!n x. Holds(R,Eval(SUC,n),x) ==> 
+  ?x0. Holds(R,n,x0) & x = Eval(f,x0)’
+ >-- (rpt strip_tac >> first_x_assum drule >>
+     pop_assum strip_assume_tac >> 
+     first_x_assum (qspecl_then [‘n’] assume_tac) >> fs[] >>
+     qexists_tac ‘r0’ >> arw[]) >>
+ x_choose_then "ss1" strip_assume_tac u_R_ss1 >>
+ pop_assum (K all_tac) >>
+ pop_assum (assume_tac o GSYM) >>
+ qby_tac 
+ ‘!n x. Holds(R,n,x) ==> IN(Pair(n,x),ss1)’
+ >-- (first_x_assum match_mp_tac >> once_arw[] >>
+      rw[Pair_def] >> strip_tac (* 2 *)
+      >-- (strip_tac (*2*)>> first_x_assum accept_tac) >>
+      rpt strip_tac (* 2 *)
+      >-- (first_x_assum irule >> first_x_assum accept_tac) >>
+      first_assum (qspecl_then [‘n'’,‘x''’] assume_tac) >>
+      first_x_assum drule >> pop_assum strip_assume_tac >> 
+      once_arw[] >>
+      qsuff_tac ‘x0 = x'’
+      >-- (strip_tac >> arw[]) >>
+      first_x_assum irule >> first_x_assum accept_tac) >>
+ pop_assum mp_tac >> once_arw[] >> rw[Pair_def] >>
+ rpt strip_tac >> 
+ qby_tac
+ ‘!n x.Holds(R,n,x) ==>
+  !x'. Holds(R,n,x') ==> x' = x’
+ >-- (rpt strip_tac >> first_assum drule >>
+      first_x_assum drule >> pop_assum strip_assume_tac >>
+      flip_tac >> first_x_assum irule >>
+      first_x_assum accept_tac) >>
+ qby_tac
+ ‘!n.?x. Holds(R,n,x)’
+ >-- (irule ex_ind_l >> rpt strip_tac >--
+     (last_x_assum drule >> qexists_tac ‘Eval(f,x)’ >> arw[]) >>
+     qexists_tac ‘a’ >> arw[]) >>
+ qby_tac
+ ‘isFun(R)’
+ >-- (rw[Fun_expand] >> arw[] >> rpt strip_tac >>
+      first_x_assum drule >> first_x_assum irule >> arw[]) >>
+ qexists_tac ‘R’ >> arw[] >>
+ drule $ GSYM Eval_def >> flip_tac >> once_arw[] >>
+ strip_tac >-- first_x_assum accept_tac >>
+ strip_tac >>
+ drule Holds_Eval >> 
+ first_x_assum (qspecl_then [‘n’] assume_tac) >> 
+ last_x_assum irule >> first_x_assum accept_tac
+ )
+(form_goal
+ “!X a:mem(X) f:X->X. isFun(f) ==>
+ ?u:N->X. isFun(u) & Eval(u,O) = a & 
+ !n:mem(N).Eval(u,Eval(SUC,n)) = Eval(f,Eval(u,n))”));
+end
+
+
+
+
+
+
+
+
+val lemma = 
+ fVar_Inst 
+[("P",([("A",mem_sort$ Pow $ Cross N (mk_set "X"))],
+“IN(Pair(O,a:mem(X)),A) &
+ (!n x.IN(Pair(n,x),A) ==> IN(Pair(Eval(SUC,n),Eval(f,x)),A))”))] 
+(IN_def_P_expand |> qspecl [‘Pow(N * X)’]) 
+
+val As_def = lemma |> ex2fsym0 "As" ["a","f"] |> conjE1 
+                   |> gen_all |> GSYM
+
+val U_ex_lemma = fVar_Inst 
+[("P",([("nx",mem_sort $ Cross N (mk_set "X"))],
+“IN(nx,Eval(BI(N * X),As(a0,f)))”))]
+(Thm_2_4 |> qspecl [‘N * X’]) 
+|> conv_rule $ once_depth_fconv no_conv 
+$ rewr_fconv (spec_all BI_property)
+|> conv_rule $ once_depth_fconv no_conv 
+$ rewr_fconv (spec_all As_def) |> gen_all
+
+val rel_ex_lemma = 
+fVar_Inst 
+[("P",([("n",mem_sort N),("x",mem_sort (mk_set "X"))],
+“?r.Eval(u0:U-> N * X,r) = Pair(n,x)”))]
+
+(AX1 |> qspecl [‘N’,‘X’]) |> uex_expand
+
+
